proof/Merges/HoareGoto/HoareGoto2_Record.v
@@ -1,0 +1,316 @@
+Require Import Merges.Tactics.
+Require Import Merges.Map.
+
+
+Require Import Merges.List.List.
+Require Import Coq.Lists.List.
+Import ListNotations.
+Set Implicit Arguments.
+
+Module Base.
+Section Goto.
+ Variable Var : Set.
+ Variable VarEqDec : EqDec Var.
+ Variable Label : Set.
+
+ Definition Value := nat.
+ Definition Heap := Map Var Value.
+ Definition Pred := Heap -> Prop.
+
+ Let varUpdate := Map.update Var Value VarEqDec.
+ Let predUpdate v f (p : Pred)
+    := fun s => p (varUpdate v (f (s v)) s).
+
+ Let predImplies (p1 p2 : Pred)
+    := forall s, p1 s -> p2 s.
+
+
+  Inductive Instr : Type :=
+   | IInc : Var -> Instr
+   | IDec : Var -> Instr
+   | INop : Instr
+  .
+  Hint Constructors Instr.
+
+  Let InstrPre (i : Instr) (post : Pred) : Pred :=
+   match i with
+   | IInc v => predUpdate v (fun n => S n)    post
+   | IDec v => predUpdate v (fun n => pred n) post
+   | INop   => post
+   end.
+
+
+
+  Inductive Block : Type :=
+     BlockJump : Label -> Instr -> Block
+   | BlockJZ   : Var -> Label -> Label -> Block
+   | BlockExit : Block.
+  Hint Constructors Block.
+
+  Variable Blocks : Label -> Block.
+  Variable LabelPre  : Label -> Pred.
+
+  Definition BlockPre (l : Label) (b : Block) : Prop :=
+    match b with
+     | BlockJump l' i
+     => predImplies (LabelPre l) (InstrPre i (LabelPre l'))
+     /\ predImplies (InstrPre i (LabelPre l')) (LabelPre l')
+
+     | BlockJZ v lz lnz
+     => predImplies (fun s => LabelPre l s /\ s v  = 0) (LabelPre lz)
+     /\ predImplies (fun s => LabelPre l s /\ s v <> 0) (LabelPre lnz)
+
+     | BlockExit
+     => True
+    end.
+  Hint Unfold BlockPre.
+
+  Hypothesis BlocksPre: forall l, BlockPre l (Blocks l).
+
+
+  Inductive EvalI : Heap -> Instr -> Heap -> Prop :=
+   | EvalIInc v s
+      : EvalI s (IInc v) (varUpdate v (S (s v)) s)
+   | EvalIDec v s
+      : EvalI s (IDec v) (varUpdate v (pred (s v)) s)
+   | EvalINop s
+      : EvalI s INop s.
+  Hint Constructors EvalI.
+
+  Inductive EvalB : Heap -> Label -> Heap -> Label -> Prop :=
+   | EvalBJump l l' i s s'
+      : Blocks l = BlockJump l' i
+     -> EvalI s i s'
+     -> EvalB s l s' l'
+   | EvalBJZ'Z v l lz lnz s
+      : Blocks l = BlockJZ v lz lnz
+     -> s v = 0
+     -> EvalB s l s lz
+   | EvalBJZ'NZ v l lz lnz s
+      : Blocks l = BlockJZ v lz lnz
+     -> s v <> 0
+     -> EvalB s l s lnz.
+
+  Theorem EvalI_Hoare i s s' post
+   (hPre : InstrPre i post s)
+   (hEvI : EvalI s i s')
+         : post s'.
+  Proof.
+   induction~ hEvI.
+  Qed.
+
+  Theorem BlockPre_Get l b
+    : Blocks l = b
+   -> BlockPre l b.
+  Proof.
+    intros.
+    rewrite <- H.
+    apply BlocksPre.
+  Qed.
+  Hint Immediate BlockPre_Get.
+
+  Theorem EvalB_Hoare l l' s s'
+   (hPre : LabelPre l s)
+   (hEvB : EvalB s l s' l')
+         : LabelPre l' s'.
+  Proof.
+   induction~ hEvB;
+    destructs~ (BlockPre_Get H).
+    eapply EvalI_Hoare; eauto.
+  Qed.
+
+
+
+  Inductive EvalBs : Heap -> Label -> Heap -> Label -> Prop :=
+   | EvalBs0 l s
+      : Blocks l = BlockExit
+     -> EvalBs s l s l
+   | EvalBs1 l s l' s' l'' s''
+      : EvalB  s l s' l'
+     -> EvalBs s' l' s'' l''
+     -> EvalBs s l s'' l''.
+
+
+  Theorem EvalBs_Hoare l l' s s'
+   (hPre : LabelPre l s)
+   (hEvB : EvalBs s l s' l')
+         : LabelPre l' s'.
+  Proof.
+   induction~ hEvB.
+    apply EvalB_Hoare in H; eauto.
+  Qed.
+End Goto.
+Section Functor.
+  Definition Instr_map_V {A B : Set} (f : A -> B) (i : Instr A) : Instr B :=
+   match i with
+   | IInc v => IInc (f v)
+   | IDec v => IDec (f v)
+   | INop _ => INop _
+   end.
+
+  Theorem Instr_map_V_id:
+    forall A i, @Instr_map_V A A id i = i.
+  Proof.
+   destruct i; eauto.
+  Qed.
+
+  Definition Block_map_V {L A B : Set} (f : A -> B) (b : Block A L) : Block B L :=
+   match b with
+   | BlockJump l i    => BlockJump l (Instr_map_V f i)
+   | BlockJZ v lz lnz => BlockJZ (f v) lz lnz
+   | BlockExit _ _    => BlockExit _ _
+   end.
+  Definition Block_map_L {V A B : Set} (f : A -> B) (b : Block V A) : Block V B :=
+   match b with
+   | BlockJump l i    => BlockJump (f l) i
+   | BlockJZ v lz lnz => BlockJZ v (f lz) (f lnz)
+   | BlockExit _ _    => BlockExit _ _
+   end.
+
+
+  Theorem Pred_map_V {A B : Set}
+      (f : A -> B)
+      (p : Pred A):
+    Pred B.
+  Proof.
+   firstorder.
+  Qed.
+End Functor.
+End Base.
+
+Module Program.
+ Module B := Base.
+
+ Record Program (Var Label : Set) : Type
+  := mkProgram
+   { VarEqDec : EqDec Var
+   ; Blocks   : Label -> B.Block Var Label
+   ; LabelPre : Label -> B.Pred Var
+   ; BlocksPre: (forall l : Label, B.BlockPre VarEqDec LabelPre l (Blocks l))
+   }.
+
+End Program.
+
+
+Module Nowt.
+  Inductive V0 : Set :=.
+  Inductive L := L1.
+
+  Definition LabelPre (l : L) (h : Base.Heap V0) := True.
+
+  Module P := Program.
+  Program Definition r := {| P.Blocks := (fun _ => Base.BlockExit V0 L); P.LabelPre := LabelPre |}.
+  Solve Obligations with prove_eqdec.
+  Solve Obligations.
+End Nowt.
+
+
+Module Zero.
+  Inductive V : Set := V1.
+  Inductive L := L0 | L1 | L2.
+
+  Module B := Base.
+  Definition Blocks (l : L) :=
+   match l with
+   | L0 => B.BlockJump L1 (B.IDec V1)
+   | L1 => B.BlockJZ V1 L2 L0
+   | L2 => B.BlockExit V L
+   end.
+  Definition LabelPre (l : L) : B.Pred V :=
+   match l with
+   | L0 => fun h => True
+   | L1 => fun h => True
+   | L2 => fun h => h V1 = 0
+   end.
+
+  Program Definition r := {| Program.Blocks := Blocks; Program.LabelPre := LabelPre |}.
+  Solve Obligations with prove_eqdec.
+  Next Obligation.
+   destruct l; firstorder.
+  Qed.
+End Zero.
+
+Module Seq.
+ Module P := Program.
+ Section Seq.
+  Variable V L1 L2 : Set.
+  Variable P1 : P.Program V L1.
+  Variable P2 : P.Program V L2.
+  Inductive L' := L'1 (l : L1) | L'2 (l : L2).
+  
+  Variable L2Start : L2.
+
+  Hypothesis L2Pre:
+    forall (l : L1),
+    P.Blocks P1 l = Base.BlockExit _ _ ->
+    (forall (h : Base.Heap V), (P.LabelPre P1 l h) -> (P.LabelPre P2 L2Start h)).
+
+  Let Jumpy
+   := Base.BlockJump (L'2 L2Start) (Base.INop V).
+
+  Definition Blocks (l : L') :=
+   match l with
+   | L'1 l1
+   => match P.Blocks P1 l1 with
+      | Base.BlockExit _ _ => Jumpy
+      | b => Base.Block_map_L (L'1) b
+      end
+   | L'2 l2 => Base.Block_map_L (L'2) (P.Blocks P2 l2)
+   end.
+
+  Definition LabelPre (l : L') :=
+   match l with
+   | L'1 l1 => P.LabelPre P1 l1
+   | L'2 l2 => P.LabelPre P2 l2
+   end.
+
+ Axiom EqDecExtensional : forall (A : Set) (m m' : EqDec A),
+   m = m'.
+
+  Program Definition r := {| P.VarEqDec := P.VarEqDec P1; P.Blocks := Blocks; P.LabelPre := LabelPre |}.
+  Next Obligation.
+    destruct l; eauto.
+    remember (P.Blocks P1 l).
+    remember (P.BlocksPre P1 l).
+    clear Heqb0.
+    rewrite <- Heqb in b0.
+
+    destruct b; eauto;
+    simpl; rewrite~ <- Heqb.
+    unfold Jumpy. simpls. eauto.
+
+    remember (P.Blocks P2 l).
+    remember (P.BlocksPre P2 l).
+    clear Heqb0.
+    rewrite <- Heqb in b0.
+    cuts_rewrite (P.VarEqDec P1 = P.VarEqDec P2).
+    destruct b; simpl; rewrite~ <- Heqb.
+
+    clear.
+    apply EqDecExtensional.
+   Qed.
+
+ End Seq.
+End Seq.
+Check Seq.L'.
+
+Set Default Goal Selector "all".
+
+(*
+
+Module Plus2.
+  Module Var <: Var.
+    Inductive Var' := VIn1 | VIn2 | VOut.
+    Definition Var := Var'.
+    Definition VarEqDec : EqDec Var.
+    Proof. prove_eqdec. Qed.
+    Definition update t := Map.update Var t VarEqDec.
+  End Var.
+
+  Module Label <: Label.
+    Inductive Var' := VIn1 | VIn2 | VOut.
+    Definition Var := Var'.
+    Definition VarEqDec : EqDec Var.
+    Proof. prove_eqdec. Qed.
+    Definition update t := Map.update Var t VarEqDec.
+*)
